Isabelle/Grammar_defs.thy
@@ -23,10 +23,10 @@ type_synonym ('t, 'v) norm_list = "('v \<times> (nat \<times> ('t, 'v) productio
 definition gram_valid :: "('t::linorder, 'v::linorder) grammar \<Rightarrow> bool" where
   "gram_valid gr \<equiv> is_typical_alist gr \<and>
      (\<forall>(v, rules) \<in> set gr. is_typical_alist rules \<and>
-       (\<forall>vs \<in> snd ` set rules. set vs \<subseteq> fst ` set gr))"
+       (\<forall>vs \<in> snd ` set rules. set vs \<subseteq> keys gr))"
 
 definition gram_max_vars :: "('t, 'v) grammar \<Rightarrow> nat" where
-  "gram_max_vars gr = Max (set (map (\<lambda>(_, rules). Max (set (map (\<lambda>(_, vs). length vs) rules))) gr))"
+  "gram_max_vars gr = Max (set (map (\<lambda>(_, rules). Max (set (map (length \<circ> snd) rules))) gr))"
 
 
 (*****************************************************************************
@@ -34,10 +34,10 @@ definition gram_max_vars :: "('t, 'v) grammar \<Rightarrow> nat" where
  *****************************************************************************)
 
 definition norm_sum :: "('t, 'v) norm_list \<Rightarrow> 'v list \<Rightarrow> nat" where
-  "norm_sum norms vars \<equiv> listsum (map fst (map (\<lambda>v. of_key norms v) vars))"
+  "norm_sum norms vars \<equiv> listsum (map (fst \<circ> lookup norms) vars)"
 
 definition rule_has_norm :: "('t, 'v) norm_list \<Rightarrow> ('t, 'v) production_rule \<Rightarrow> bool" where
-  "rule_has_norm norms \<equiv> \<lambda>(t, vs). \<forall>v \<in> set vs. v \<in> fst ` set norms"
+  "rule_has_norm norms \<equiv> \<lambda>(t, vs). \<forall>v \<in> set vs. v \<in> keys norms"
 
 definition rules_have_norm :: "('t, 'v) norm_list \<Rightarrow> ('t, 'v) production_rules \<Rightarrow> bool" where
   "rules_have_norm norms rules \<equiv> \<exists>r \<in> set rules. rule_has_norm norms r"
@@ -75,9 +75,9 @@ function minimal_word_of_variables ::
   "('t :: linorder, 'v :: linorder) grammar \<Rightarrow> 'v list \<Rightarrow> 't list" where
   "minimal_word_of_variables gr [] = []"
 | "minimal_word_of_variables gr (vh#vt) = (
-     if gram_valid (* TODO! use gram_normed here! *) gr \<and> set (vh#vt) \<subseteq> fst ` set gr then
+     if gram_valid (* TODO! use gram_normed here! *) gr \<and> set (vh#vt) \<subseteq> keys gr then
        let norms = norms_of_grammar gr in
-       let (t, vars) = snd (of_key norms vh) in
+       let (t, vars) = snd (lookup norms vh) in
        t # minimal_word_of_variables gr vars @ minimal_word_of_variables gr vt
      else [])"
 by pat_completeness auto
@@ -89,8 +89,8 @@ by pat_completeness auto
 
 fun eat_word :: "('t, 'v) grammar \<Rightarrow> 't list \<Rightarrow> 'v list \<Rightarrow> ('t list \<times> 'v list)" where
   "eat_word gr (th#tt) (vh#vt) = (
-     let prods = of_key gr vh in
-     if th \<in> fst ` set prods then eat_word gr tt ((of_key prods th) @ vt)
+     let prods = lookup gr vh in
+     if th \<in> keys prods then eat_word gr tt ((lookup prods th) @ vt)
      else (th#tt, vh#vt))"
 | "eat_word gr t v = (t, v)"
 
@@ -125,7 +125,7 @@ fun norm_reduce :: "('t :: linorder, 'v :: linorder) grammar \<Rightarrow> 'v li
   "norm_reduce gr v 0 = v"
 | "norm_reduce gr [] (Suc p) = []"
 | "norm_reduce gr (vh#vt) (Suc p) = (
-     let (n, (_, v)) = of_key (norms_of_grammar gr) vh in
+     let (n, (_, v)) = lookup (norms_of_grammar gr) vh in
      if Suc p < n then (norm_reduce gr v p) @ vt
      else norm_reduce gr vt (Suc p - n))"
 
